forgot

Arith/AST.lean
@@ -1,29 +1,21 @@
-inductive Op0 where
-  | peekbyte
-  | readbyte
-deriving Repr
+import «Arith».Types
+open Convertible
 
 inductive Op1 where
   | add1
   | sub1
-  | zeroHuh
-  | charHuh
-  | inttochar
-  | chartoint
-  | writeByte
-  | eofobjecthuh
+  | intToChar
+  | charToInt
   | neg
+  | not
   | abs
-  | inthuh
-  | boolhuh
 deriving Repr
 
 inductive Op2 where
+  | plus
   | sub
-deriving Repr
-
-inductive OpN where
-  | add
+  | lt
+  | eq
 deriving Repr
 
 abbrev ID := String
@@ -32,12 +24,11 @@ inductive Expr where
   | integer (n : Nat)
   | boolean (b : Bool)
   | character (c : Char)
-  | prim0  (op : Op0)
   | prim1  (op : Op1) (e : Expr)
   | prim2  (op : Op2) (e1 : Expr) (e2 : Expr)
-  | primn  (op : OpN) (es : List Expr)
-  | letstd (ids : List ID) (es : List Expr) (body : Expr)
-  | letstar (ids : List ID) (es : List Expr) (body : Expr)
+  | letstd (id : ID) (es : Expr) (body : Expr)
   | begin  (e1 : Expr) (e2 : Expr)
   | var (id : ID)
+  | if (e1 : Expr) (e2 : Expr) (e3: Expr)
+
 deriving Repr
