Arith/Compile.lean
@@ -15,14 +15,11 @@ abbrev Context := List (ID × Reg)
   let r' <- get
   set (next r')
   return [
-    mov r' r, 
+    mov r' r,
     and r' mask,
     cmpi r' type,
     haltne
   ]
-
-@[simp] def typePred (mask : Nat) (type : Nat) : Prog :=
-  [and rax mask, cmpi rax type, mov rax (valToBits true), je 1, mov rax (valToBits false)]
 
 @[simp] def assertInteger := assertType int_mask type_int
 
@@ -33,17 +30,28 @@ abbrev Context := List (ID × Reg)
   return (
     check ++
    [cmpi r (valToBits 0),
-    haltl, 
+    haltl,
     cmpi rax (valToBits 1114111),
-    haltg, 
+    haltg,
     cmpi rax (valToBits 55295),
     jl 3,
     cmpi rax (valToBits 57344),
     jg 1,
-    halt 
+    halt
    ])
 
-@[simp] def compileVal (val : α) [Convertible α] : Prog := 
+@[simp] def eqImm (imm : Nat) : Prog :=
+  [
+    cmpi rax imm,
+    mov rax val_true,
+    je 1,
+    mov rax val_false
+  ]
+
+@[simp] def compileBits (val : Nat) : Prog :=
+  [movi rax val]
+
+@[simp] def compileVal (val : α) [Convertible α] : Prog :=
   [movi rax (valToBits val)]
 
 @[simp] def compile_op1 (op : Op1) : StateT Reg (Except String) Prog :=
@@ -54,37 +62,89 @@ abbrev Context := List (ID × Reg)
   | .sub1 => do
       let check <- assertInteger rax
       return (check ++ [subi rax (valToBits 1)])
-  -- | .zerohuh => do
-  --     let check <- assertInteger rax
-  --     return (
-  --       check ++ 
-  --      [cmpi rax 0,
-  --       movi rax val_true,
-  --       je 1,
-  --       movi rax val_false])
-  -- | .charhuh => return (typePred char_mask type_char)
-  -- | .chartoint => do
-  --     let check <- assertChar rax
-  --     return (
-  --       check ++
-  --      [sar rax char_shift,
-  --       sal rax int_shift])
-  -- | .inttochar => do
-  --     let check <- assertCodepoint rax
-  --     return (
-  --       check ++ 
-  --      [sar rax int_shift,
-  --       sal rax char_shift,
-  --       xor rax type_char])
-  -- | .neg => do
-  --     let check <- assertInteger rax
-  --     let r <- get
-  --     set (next r)
-  --     return 
+  | .charToInt => do
+      let check <- assertChar rax
+      return (
+        check ++
+       [sar rax char_shift,
+        sal rax int_shift])
+  | .intToChar => do
+      let check <- assertCodepoint rax
+      return (
+        check ++
+       [sar rax int_shift,
+        sal rax char_shift,
+        xor rax type_char])
+  | .neg => do
+      let check <- assertInteger rax
+      let r <- get
+      set (next r)
+      return (
+        check ++
+        [mov r 0,
+         sub r rax,
+         mov rax r])
+  | .abs => do
+      let check <- assertInteger rax
+      let r <- get
+      set (next r)
+      return (
+        check ++
+        [cmpi rax 0,
+         jg 3,
+         mov r 0,
+         sub r rax,
+         mov rax r
+      ])
+  | .not =>
+      return [
+        cmp rax val_false,
+        mov rax val_true,
+        je 1,
+        mov rax val_false
+      ]
 
-  | _ => return []
+def compile_op2 (op: Op2) (prev : Reg): StateT Reg (Except String) Prog :=
+  match op with
+  | .plus => do
+    let check <- assertInteger prev
+    let check' <- assertInteger rax
+    return (
+      check ++
+      check' ++
+      [add prev rax,
+        mov rax prev])
+  | .sub => do
+    let check <- assertInteger prev
+    let check' <- assertInteger rax
+    return (
+      check ++
+      check' ++
+      [sub prev rax,
+        mov rax prev])
+  | .lt => do
+    let check <- assertInteger prev
+    let check' <- assertInteger rax
+    return (
+      check ++
+      check' ++
+      [cmp prev rax,
+       mov rax val_true,
+       jl 1,
+       mov rax val_false]
+    )
+  | .eq => do
+    let check <- assertInteger prev
+    let check' <- assertInteger rax
+    return (
+      check ++
+      check' ++
+      [cmp prev rax,
+       mov rax val_true,
+       je 1,
+       mov rax val_false]
+    )
 
-mutual
 @[simp] def compile_expr (e : Expr) (c : Context) : StateT Reg (Except String) Prog :=
   match e with
   | .integer n    => return (compileVal n)
@@ -97,22 +157,35 @@ mutual
       let instrs <- compile_expr e c
       let instrs' <- compile_op1 op
       return (instrs ++ instrs')
-  | .letstd ids es body => do
-      let (regs, progs) <- compile_star es c
-      let prog <- compile_expr body ((List.zip ids regs) ++ c)
-      return (progs ++ prog)
-  | _ => return [mov rax 1]
-
-@[simp] def compile_star (es : List Expr) (c : Context) : StateT Reg (Except String) ((List Reg) × Prog) :=
-  match es with
-  | []    => return ([], [])
-  | e::es => do
-      let e_instrs <- compile_expr e c
+  | .prim2 op e1 e2 => do
+      let instrs <- compile_expr e1 c
       let r <- get
       set (next r)
-      let (rs, es_instrs) <- compile_star es c
-      return (r::rs, e_instrs ++ [mov r rax] ++ es_instrs)
-end
+      let instrs' <- compile_expr e2 c
+      let instrs'' <- compile_op2 op r
+      return (instrs ++ [mov r rax] ++ instrs' ++ instrs'')
+  | .if e1 e2 e3 => do
+      let instrs <- compile_expr e1 c
+      let instrs' <- compile_expr e2 c
+      let instrs'' <- compile_expr e3 c
+      return (
+        instrs ++
+        [cmp rax val_false,
+        je (List.length instrs' + 1)] ++
+        instrs' ++
+        [jmp (List.length instrs'')] ++
+        instrs''
+      )
+  | .begin e1 e2 => do
+      let instrs <- compile_expr e1 c
+      let instrs' <- compile_expr e2 c
+      return instrs ++ instrs'
+  | .letstd id e body => do
+      let instrs <- compile_expr e c
+      let r <- get
+      set (next r)
+      let instrs' <- compile_expr body ((id, r)::c)
+      return (instrs ++ [mov r rax] ++ instrs')
 
 @[simp] def compile (e : Expr) : Except String Prog :=
   match (compile_expr e [] first) with
