Arith/Instrs.lean
@@ -1,23 +1,6 @@
 import Arith.Types
 
 abbrev Reg := Nat
--- def Reg := Nat
-
--- instance : OfNat Reg 0 where
---   ofNat := Nat.zero
-
--- instance : OfNat Reg n where
---   ofNat := n
-
--- instance : Repr Reg where
---   reprPrec : Reg -> Nat -> Std.Format
---   | 0, _ => "rax"
---   | r, _ => "r" ++ (Nat.repr r)
-
--- instance : ToString Reg where
---   toString : Reg -> String
---   | 0 => "rax"
---   | r => "r" ++ (Nat.repr r)
 
 instance : BEq Reg where
   beq := Nat.beq
@@ -69,64 +52,6 @@ inductive Instr : Type
 deriving Repr, BEq
 
 abbrev Prog := List Instr
-open Instr
-mutual
-  @[simp] def exec1 (prog : Prog) (c : Config) : Prog × Config :=
-    match c with
-    | (acc, flag, prog_count, mem) => (match prog with
-      | [] => (prog, c)
-      | (mov r1 0)::ps      => exec1 ps (acc, flag, prog_count + 1, set r1 acc mem)
-      | (mov 0 r2)::ps      => exec1 ps (get r2 mem, flag, prog_count + 1, mem)
-      | (mov r1 r2)::ps     => exec1 ps (acc, flag, prog_count + 1, set r1 (get r2 mem) mem)
-      | (movi 0 imm)::ps    => exec1 ps (imm, flag, prog_count + 1, mem)
-      | (movi r1 imm)::ps   => exec1 ps (acc, flag, prog_count + 1, set r1 imm mem)
-      | (addi 0 imm)::ps    => exec1 ps (acc + imm, flag, prog_count + 1, mem)
-      | (addi r1 imm)::ps   => exec1 ps (acc, flag, prog_count + 1, set r1 ((get r1 mem) + imm) mem)
-      | (subi 0 imm)::ps    => exec1 ps (acc - imm, flag, prog_count + 1, mem)
-      | (subi r1 imm)::ps   => exec1 ps (acc, flag, prog_count + 1, set r1 ((get r1 mem) - imm) mem)
-      | (add 0 r2)::ps      => exec1 ps (acc + get r2 mem, flag, prog_count + 1, mem)
-      | (add r1 0)::ps      => exec1 ps (acc, flag, prog_count + 1, set r1 (get r1 mem + acc) mem)
-      | (add r1 r2)::ps     => exec1 ps (acc, flag, prog_count + 1, set r1 ((get r1 mem) + (get r2 mem)) mem)
-      | (sub 0 r2)::ps      => exec1 ps (acc - get r2 mem, flag, prog_count + 1, mem)
-      | (sub r1 0)::ps      => exec1 ps (acc, flag, prog_count + 1, set r1 (get r1 mem - acc) mem)
-      | (sub r1 r2)::ps     => exec1 ps (acc, flag, prog_count + 1, set r1 ((get r1 mem) - (get r2 mem)) mem)
-      | (Instr.xor rax imm)::ps   => exec1 ps (acc ^^^ imm, flag, prog_count + 1, mem)
-      | (Instr.and 0 imm)::ps     => exec1 ps (acc &&& imm, flag, prog_count + 1, mem)
-      | (Instr.and r1 imm)::ps    => exec1 ps (acc, flag, prog_count + 1, set r1 (get r1 mem &&& imm) mem)
-      | (sar rax imm)::ps   => exec1 ps (acc >>> imm, flag, prog_count + 1, mem)
-      | (sal rax imm)::ps   => exec1 ps (acc <<< imm, flag, prog_count + 1, mem)
-      | (cmp 0 r2)::ps      =>
-          let v := get r2 mem
-          let flag' := if (acc == v) then 0 else (if acc < v then 1 else 2)
-          exec1 ps (acc, flag', prog_count + 1, mem)
-      | (cmp r1 r2)::ps     =>
-          let v1 := get r1 mem
-          let v2 := get r2 mem
-          let flag' := if (v1 == v2) then 0 else (if v1 < v2 then 1 else 2)
-          exec1 ps (acc, flag', prog_count + 1, mem)
-      | (cmpi 0 imm)::ps    =>
-          let flag' := if (acc == imm) then 0 else (if acc < imm then 1 else 2)
-          exec1 ps (acc, flag', prog_count + 1, mem)
-      | (cmpi r1 imm)::ps   =>
-          let v := get r1 mem
-          let flag' := if (v == imm) then 0 else (if v < imm then 1 else 2)
-          exec1 ps (acc, flag', prog_count + 1, mem)
-      | (jmp n)::ps         => jump_forward ps c n
-      | (je n)::ps          => if flag == 0 then jump_forward ps c n else exec1 ps (acc, flag, prog_count + 1, mem) -- other instructions
-      | (jne n)::ps         => if flag != 0 then jump_forward ps c n else exec1 ps (acc, flag, prog_count + 1, mem)
-      | (jl n)::ps          => if flag == 1 then jump_forward ps c n else exec1 ps (acc, flag, prog_count + 1, mem)
-      | (jg n)::ps          => if flag == 2 then jump_forward ps c n else exec1 ps (acc, flag, prog_count + 1, mem)
-      | halt::ps            => (ps, (acc, flag, prog_count, mem))
-      | halteq::ps          => if flag == 0 then (ps, (acc, flag, prog_count, mem)) else exec1 ps (acc, flag, prog_count + 1, mem)
-      | haltne::ps          => if flag != 0 then (ps, (acc, flag, prog_count, mem)) else exec1 ps (acc, flag, prog_count + 1, mem)
-      | haltl::ps           => if flag == 1 then (ps, (acc, flag, prog_count, mem)) else exec1 ps (acc, flag, prog_count + 1, mem)
-      | haltg::ps           => if flag == 2 then (ps, (acc, flag, prog_count, mem)) else exec1 ps (acc, flag, prog_count + 1, mem))
-  @[simp] def jump_forward (prog : Prog) (c : Config) (n : Nat) : Prog × Config :=
-    match prog, n, c with
-    | [], _, _                                            => ([], c)
-    | ps, 0, (acc, flag, prog_count, mem)                 => exec1 ps (acc, flag, prog_count + 1, mem)
-    | _::ps, Nat.succ n', (acc, flag, prog_count, mem)    => jump_forward ps (acc, flag, prog_count + 1, mem) n'
-end
 
 inductive SmallStep : Instr -> Config -> Config -> Prop
 | mov {acc flag i mem} (r1 : Reg) (r2 : Reg):
@@ -243,8 +168,6 @@ inductive SmallStep : Instr -> Config -> Config -> Prop
 | haltg_ne {acc flag i mem} (hcond : flag != 2):
   SmallStep (Instr.haltg) (acc, flag, i, mem) (acc, flag, i + 1, mem)
 
-
-@[simp] def exec (prog : Prog) : Nat :=
-  match exec1 prog (0, 0, 0, empty) with
-  | ([], c) => c.fst
-  | (_, _)  => val_void
+inductive exec2 : Prog -> Config -> Config -> Prop
+| exec2 {prog instr acc flag mem c'} {i : Nat} (hnth : prog.get? n = some instr) (hstep : SmallStep instr (acc, flag, i, mem) c'):
+    exec2 prog (acc, flag, i, mem) c'
