Arith/Example.lean
@@ -5,4 +5,4 @@ open OpN
 open Op1
 open Op2
 
-def exampl : Expr := letstd ["x","y"] [integer 1,integer 2] (var "x")
+def exampl : Expr :=var "x"
