Arith/Stack.lean
@@ -1,0 +1,93 @@
+inductive instr where
+| Push (n : Int)
+| Plus
+| Minus
+deriving Repr
+
+inductive aexp where
+  | integer (n : Int)
+  | plus (a1 a2 : aexp)
+  | minus (a1 a2 : aexp)
+  | add1 (a1 : aexp)
+  | sub1 (a1 : aexp)
+  | neg (a1 : aexp)
+
+def aeval (e : aexp) : Int :=
+  match e with
+  | .integer n => n
+  | .plus a1 a2 => (aeval a1) + (aeval a2)
+  | .minus a1 a2 => (aeval a1) - (aeval a2)
+  | .add1 a1 => (aeval a1) + 1
+  | .sub1 a1 => (aeval a1) - 1
+  | .neg a1 =>  0 - (aeval a1)
+
+
+@[simp] def stackExecA (stack : List Int) (prog : List instr) : List Int :=
+  match prog with
+  | [] => stack
+  | .Push n::ps => stackExecA (n::stack) ps
+  | .Plus::ps =>
+      match stack with
+      | n1::n2::xs => stackExecA ((n2 + n1)::xs) ps
+      | _ => stackExecA stack ps
+  | .Minus::ps =>
+      match stack with
+      | n1::n2::xs => stackExecA ((n2 - n1)::xs) ps
+      | _ => stackExecA stack ps
+
+open instr
+open aexp
+@[simp] def stackCompile (e : aexp) : List instr :=
+  match e with
+  | .integer n => [Push n]
+  | .plus a1 a2 => (stackCompile a1) ++ (stackCompile a2) ++ [Plus]
+  | .minus a1 a2 => (stackCompile a1) ++ (stackCompile a2) ++ [Minus]
+  | .add1 a1 => (stackCompile a1) ++ [Push 1, Plus]
+  | .sub1 a1 => (stackCompile a1) ++ [Push 1, Minus]
+  | .neg a1 => [Push 0] ++ (stackCompile a1) ++ [Minus]
+
+theorem executeAppend (p1 p2 : List instr) (stack : List Int) :
+  stackExecA stack (p1 ++ p2) = stackExecA (stackExecA stack p1) p2 :=
+  by
+  revert stack
+  revert p2
+  induction p1 with
+  intros p2 stack
+  | nil => rfl
+  | cons a p1 IHp1 =>
+    cases a <;>
+    simp <;>
+    repeat (
+      cases stack
+      case nil => apply IHp1
+      case cons _ stack => cases stack <;> try apply IHp1)
+
+theorem stackCompileCorrectH (stack : List Int) (e : aexp) :
+  stackExecA stack (stackCompile e) = aeval e :: stack :=
+  by
+    revert stack
+    induction e with
+    intro stack <;> simp
+    | integer n =>
+      rfl
+    | plus e1 e2 IHe1 IHe2 =>
+      repeat (rewrite [executeAppend])
+      rewrite [IHe1, IHe2]
+      rfl
+    | minus e1 e2 IHe1 IHe2 =>
+      repeat (rewrite [executeAppend])
+      rewrite [IHe1, IHe2]
+      rfl
+    | add1 e1 IHe1 =>
+      rewrite [executeAppend, IHe1]
+      rfl
+    | sub1 e1 IHe1 =>
+      rewrite [executeAppend, IHe1]
+      rfl
+    | neg e1 IHe1 =>
+      rewrite [executeAppend, IHe1]
+      rfl
+
+theorem stackCompileCorrect (stack : List Int) (e : aexp) :
+  stackExecA [] (stackCompile e) = [aeval e] :=
+  by apply stackCompileCorrectH
