Arith/Types.lean
@@ -1,25 +1,25 @@
-def int_shift := 1
-def char_shift := 2
-def val_true := 3
-def val_false := 7
-def val_void := 15
+@[simp] def int_shift := 1
+@[simp] def char_shift := 2
+@[simp] def val_true := 3
+@[simp] def val_false := 7
+@[simp] def val_void := 15
 
-def type_char := 1
-def type_int := 0
+@[simp] def type_char := 1
+@[simp] def type_int := 0
 
-def int_mask := 1
-def char_mask := 3
+@[simp] def int_mask := 1
+@[simp] def char_mask := 3
 
 class Convertible (α : Type) where
   valToBits : α → Nat
 
-instance : Convertible Nat where
+@[simp] instance : Convertible Nat where
   valToBits v := v <<< int_shift
 
-instance : Convertible Bool where
+@[simp] instance : Convertible Bool where
   valToBits : Bool -> Nat
   | true => val_true
   | false => val_false
 
-instance : Convertible Char where
+@[simp] instance : Convertible Char where
   valToBits v := ((Char.toNat v) <<< char_shift) ||| type_char
